Solution of ex6d

doc/tutorial/code/solutions/ex6d-no-discard.fst
@@ -1,100 +1,105 @@
-module QuicksortNoDiscard
+module QuickSortNoDiscard
+
+
+(* Instead of a Boolean check that an element belongs to a list, count
+the number of occurrences of an element in a list *)
+val count : 'a -> list 'a -> Tot nat
+let rec count (x:'a) (l:list 'a) = match l with
+  | hd::tl -> if hd=x then 1 + count x tl else count x tl
+  | [] -> 0
+
+let mem x l = count x l > 0
+
 
 val append : list 'a -> list 'a -> Tot (list 'a)
 let rec append l1 l2 = match l1 with
   | [] -> l2
   | hd :: tl -> hd :: append tl l2
 
+
+val append_count: l:list 'a -> m:list 'a
+               -> Lemma (requires True)
+                        (ensures (forall x. count x (append l m) = (count x l + count x m)))
+let rec append_count l m = match l with
+  | [] -> ()
+  | hd::tl -> append_count tl m
+
+
+val append_mem: l:list 'a -> m:list 'a
+               -> Lemma (requires True)
+                        (ensures (forall x. mem x (append l m) = (mem x l || mem x m)))
+let append_mem l m = append_count l m
+
+
 val length: list 'a -> Tot nat
 let rec length l = match l with
   | [] -> 0
   | _ :: tl -> 1 + length tl
 
-val partition: ('a -> Tot bool) -> list 'a -> Tot (list 'a * list 'a)
-let rec partition f = function 
-  | [] -> [], []
-  | hd::tl -> 
-    let l1, l2 = partition f tl in
-    if f hd 
-    then hd::l1, l2
-    else l1, hd::l2
 
 (* Specification of sortedness according to some comparison function f *)
 val sorted: ('a -> 'a -> Tot bool) -> list 'a -> Tot bool
-let rec sorted f = function
-  | []
-  | [_] -> true
-  | x::y::tl -> f x y && sorted f (y::tl)
+let rec sorted f l = match l with
+    | [] -> true
+    | [x] -> true
+    | x::y::xs -> f x y && sorted f (y::xs)
 
-val count : 'a -> list 'a -> Tot nat
-let rec count (x:'a) (l:list 'a) = match l with
-  | hd::tl -> if hd=x then 1 + count x tl else count x tl
-  | [] -> 0
 
-val count_append: l:list 'a -> m:list 'a -> x:'a 
-               -> Lemma (requires True)
-                        (ensures (count x (append l m) = (count x l + count x m)))
-                        [SMTPat (count x (append l m))]
-let rec count_append l m x = match l with 
-  | [] -> ()
-  | hd::tl -> count_append tl m x
+val partition: ('a -> Tot bool) -> list 'a -> Tot (list 'a * list 'a)
+let rec partition f = function
+  | [] -> [], []
+  | hd::tl ->
+     let l1, l2 = partition f tl in
+     if f hd
+     then hd::l1, l2
+     else l1, hd::l2
 
-let mem x l = count x l > 0
 
-val append_mem:  l1:list 'a
-              -> l2:list 'a
-              -> a:'a
-              -> Lemma (requires True)
-                       (ensures (mem a (append l1 l2) = (mem a l1 || mem a l2)))
-                       [SMTPat (mem a (append l1 l2))]
-let rec append_mem l1 l2 a = match l1 with
-  | [] -> ()
-  | hd::tl -> append_mem tl l2 a
-
-(* A lemma about List.partition ... duh *)
 val partition_lemma: f:('a -> Tot bool)
-                  -> l:list 'a
-                  -> Lemma (requires True)
-                           (ensures ((fun l1 l2 -> 
-                                     (length l1 + length l2 = length l
-                                      /\ (forall x. mem x l1 ==> f x)
-                                      /\ (forall x. mem x l2 ==> not (f x))
-                                      /\ (forall x. count x l = (count x l1 + count x l2))))
-                                        (fst (partition f l))
-                                        (snd (partition f l))))
-                           (* [SMTPat (partition f l)] (\* injected to the solver *\) *)
-let rec partition_lemma f l = match l with 
-  | [] -> ()
-  | hd::tl -> partition_lemma f tl
+                   -> l:list 'a
+                   -> Lemma (requires True)
+                            (ensures ((length (fst (partition f l)) + length (snd (partition f l)) = length l
+                                  /\ (forall x. mem x (fst (partition f l)) ==> f x)
+                                  /\ (forall x. mem x (snd (partition f l)) ==> not (f x))
+                                  /\ (forall x. mem x l = (mem x (fst (partition f l)) || mem x (snd (partition f l))))
+                                  /\ (forall x. count x l = (count x (fst (partition f l)) + count x (snd (partition f l)))))))
+let rec partition_lemma f l = match l with
+    | [] -> ()
+    | hd::tl -> partition_lemma f tl
 
 
+(* Defining a new predicate symbol *)
 opaque type total_order (a:Type) (f: (a -> a -> Tot bool)) =
     (forall a. f a a)                                           (* reflexivity   *)
     /\ (forall a1 a2. (f a1 a2 /\ a1<>a2)  <==> not (f a2 a1))  (* anti-symmetry *)
     /\ (forall a1 a2 a3. f a1 a2 /\ f a2 a3 ==> f a1 a3)        (* transitivity  *)
 
-val sorted_concat_lemma:  a:Type
-               ->  f:(a -> a -> Tot bool)
-               ->  l1:list a{sorted f l1}
-               ->  l2:list a{sorted f l2}
-               ->  pivot:a
-               ->  Lemma (requires (total_order a f
-                                    /\ (forall y. mem y l1 ==> not(f pivot y))
-                                    /\ (forall y. mem y l2 ==> f pivot y))
-)                         (ensures (sorted f (append l1 (pivot::l2))))
-                          [SMTPat (sorted f (append l1 (pivot::l2)))]
-let rec sorted_concat_lemma f l1 l2 pivot = match l1 with 
-  | [] -> ()
-  | hd::tl -> sorted_concat_lemma f tl l2 pivot
+val sorted_concat_lemma: a:Type
+                      -> f:(a -> a -> Tot bool)
+                      -> l1:list a{sorted f l1}
+                      -> l2:list a{sorted f l2}
+                      -> pivot:a
+                      -> Lemma (requires (total_order a f
+                                       /\ (forall y. mem y l1 ==> not (f pivot y))
+                                       /\ (forall y. mem y l2 ==> f pivot y)))
+                               (ensures (sorted f (append l1 (pivot::l2))))
+let rec sorted_concat_lemma f l1 l2 pivot = match l1 with
+    | [] -> ()
+    | hd::tl -> sorted_concat_lemma f tl l2 pivot
 
 
 val sort: f:('a -> 'a -> Tot bool){total_order 'a f}
-      ->  l:list 'a
-      ->  Tot (m:list 'a{sorted f m /\ (forall x. count x l = count x m)})
+       -> l:list 'a
+       -> Tot (m:list 'a{sorted f m /\ (forall i. mem i l = mem i m) /\ (forall i. count i l = count i m)})
               (decreases (length l))
-let rec sort f = function
+let rec sort f l = match l with
   | [] -> []
-  | pivot::tl -> 
-    let hi, lo  = partition (f pivot) tl in 
+  | pivot::tl ->
+    let hi, lo = partition (f pivot) tl in
     partition_lemma (f pivot) tl;
-    sort f (append lo (Cons pivot (sort f hi)))
+    let lo' = sort f lo in
+    let hi' = sort f hi in
+    append_count lo' (pivot::hi');
+    append_mem lo' (pivot::hi');
+    sorted_concat_lemma f lo' hi' pivot;
+    append lo' (pivot::hi')
